src/goose_lang/lib/slice/typed_slice.v
@@ -398,6 +398,21 @@ Proof.
   rewrite !app_length !drop_length !fmap_length.
   word.
 Qed.
+
+Lemma wp_SliceCopy_full_typed stk E sl t q vs dst vs' :
+  {{{ own_slice_small sl t q vs ∗ own_slice_small dst t 1 vs' ∗ ⌜length vs = length vs'⌝}}}
+    SliceCopy t (slice_val dst) (slice_val sl) @ stk; E
+  {{{ RET #(U64 (length vs)); own_slice_small sl t q vs ∗ own_slice_small dst t 1 vs }}}.
+Proof.
+  iIntros (Φ) "(Hsrc & Hdst & %Hlen) HΦ".
+  wp_apply (wp_SliceCopy with "[$Hsrc $Hdst]"); [word|].
+  iIntros "(? & ?)".
+  rewrite Hlen.
+  rewrite drop_all.
+  list_simplifier.
+  iApply "HΦ".
+  iFrame.
+Qed.
 Opaque SliceCopy.
 
 Lemma wp_SliceAppend_to_zero stk E t `{!IntoValForType V t} v (x: val) :
