src/program_proof/chat/full/lib.v
@@ -1,0 +1,182 @@
+From Perennial.program_proof Require Import grove_prelude.
+From Goose.github_com.mit_pdos.secure_chat Require Import full.
+From iris.unstable.base_logic Require Import mono_list.
+
+Module msgT.
+Record t :=
+  mk {
+    body: u64
+  }.
+End msgT.
+
+Section lib.
+
+Context `{!heapGS Σ, !mono_listG msgT.t Σ}.
+
+Definition lockR_ChatCli γ (P : list msgT.t → iProp Σ) cp : iProp Σ :=
+  ∃ (lg : Slice.t) (lloc : list loc) (lmsg : list msgT.t),
+  (* Note: need □ P so Get() can simultaneously
+  close lock inv and return P. *)
+  "#HP" ∷ □ P lmsg ∗
+  "Hl_auth" ∷ mono_list_auth_own γ 1 lmsg ∗
+  "Hlg" ∷ cp ↦[ChatCli :: "log"] lg ∗
+  "Hsl" ∷ own_slice lg ptrT 1 lloc ∗
+  "#Hsep" ∷ ([∗ list] x1;x2 ∈ lloc;lmsg,
+    readonly (x1 ↦[msgT :: "body"] #x2.(msgT.body))).
+
+Definition is_ChatCli γ P cp : iProp Σ :=
+  ∃ (lk : loc),
+  "#Hlk" ∷ readonly (cp ↦[ChatCli :: "lock"] #lk) ∗
+  "#Hlk_inv" ∷ is_lock nroot #lk (lockR_ChatCli γ P cp).
+
+Lemma wp_init P :
+  {{{
+    (* Note: need □ P to establish lock inv with □ P. *)
+    "#HP" ∷ □ P []
+  }}}
+  Init #()
+  {{{
+    γ cp,
+    RET #cp;
+    "#Htriv_lb" ∷ mono_list_lb_own γ [] ∗
+    "#Hcli" ∷ is_ChatCli γ P cp
+  }}}.
+Proof.
+  rewrite /Init.
+  iIntros (Φ) "H HΦ".
+  iNamed "H".
+
+  wp_apply wp_allocStruct; [val_ty|].
+  iIntros (cp) "Hcli".
+  iDestruct (struct_fields_split with "Hcli") as "H".
+  iNamed "H".
+
+  wp_apply wp_NewSlice.
+  iIntros (lg) "Hsl".
+  wp_storeField.
+
+  iMod (mono_list_own_alloc []) as (γ) "(Hauth & Hlb)".
+  iAssert (lockR_ChatCli _ P _) with "[log Hsl Hauth]" as "HR".
+  {
+    rewrite /lockR_ChatCli.
+    iExists _, _, _.
+    iFrame.
+    naive_solver.
+  }
+
+  wp_apply (newlock_spec nroot with "[HR]").
+  1: iApply "HR".
+  iIntros (?) "#Hlk_inv".
+  wp_storeField.
+
+  iApply "HΦ".
+  iFrame.
+  rewrite /is_ChatCli.
+  iMod (readonly_alloc_1 with "lock") as "#Hlk".
+  iExists _.
+  by iFrame "#".
+Qed.
+
+Lemma wp_put cp γ P p m lmsg :
+  {{{
+    "Hcli" ∷ is_ChatCli γ P cp ∗
+    "#Hm" ∷ readonly (p ↦[msgT :: "body"] #m.(msgT.body)) ∗
+    "#Hl_lb" ∷ mono_list_lb_own γ lmsg ∗
+    (* Note: need □ on fupd RHS to establish lock inv with □ P. *)
+    "Hfupd" ∷ (∀ l', ⌜lmsg `prefix_of` l'⌝ -∗ P l' ={⊤}=∗ □ P (l' ++ [m]))
+  }}}
+  ChatCli__Put #cp #p
+  {{{ RET #(); True }}}.
+Proof.
+  iIntros (Φ) "H HΦ".
+  iNamed "H".
+  rewrite /ChatCli__Put.
+  rewrite /is_ChatCli.
+  iNamed "Hcli".
+  wp_apply (wp_loadField_ro with "[$]").
+
+  wp_apply (acquire_spec with "[$]").
+  iIntros "(Hlocked & HR)".
+  rewrite /lockR_ChatCli.
+  iNamed "HR".
+
+  wp_loadField.
+  wp_apply (wp_SliceAppend with "[$]").
+  iIntros (lg') "Hsl".
+  wp_storeField.
+  wp_loadField.
+
+  iDestruct (mono_list_auth_lb_valid with "[$] [$]") as %[_ Hpref].
+  iDestruct ("Hfupd" $! lmsg0 Hpref with "[$]") as "> Hfupd".
+  iMod (mono_list_auth_own_update_app [m] with "[$]") as "(Hl_auth & _)".
+
+  wp_apply (release_spec with "[-HΦ $Hlk_inv $Hlocked]").
+  {
+    iExists _, _, _.
+    iFrame "#∗".
+    naive_solver.
+  }
+
+  wp_pures.
+  by iApply "HΦ".
+Qed.
+
+Lemma wp_get cp γ P lold :
+  {{{
+    "Hcli" ∷ is_ChatCli γ P cp ∗
+    "#Hlold_lb" ∷ mono_list_lb_own γ lold
+  }}}
+  ChatCli__Get #cp
+  {{{
+    (lg : Slice.t) (lloc : list loc) (lmsg : list msgT.t),
+    RET (slice_val lg);
+    "#Hl_lb" ∷ mono_list_lb_own γ lmsg ∗
+    "Hsl" ∷ own_slice_small lg ptrT 1 lloc ∗
+    "%Hpref" ∷ ⌜lold `prefix_of` lmsg⌝ ∗
+    "HP" ∷ P lmsg ∗
+    "#Hsep" ∷ ([∗ list] x1;x2 ∈ lloc;lmsg,
+      readonly (x1 ↦[msgT :: "body"] #x2.(msgT.body)))
+  }}}.
+Proof.
+  iIntros (Φ) "H HΦ".
+  iNamed "H".
+  iNamed "Hcli".
+  rewrite /ChatCli__Get.
+
+  wp_apply (wp_loadField_ro with "[$]").
+  wp_apply (acquire_spec with "[$]").
+  iIntros "(Hlocked & H)".
+  iNamed "H".
+  wp_loadField.
+  wp_apply wp_slice_len.
+  iDestruct (own_slice_sz with "[$]") as %Hlen.
+  wp_apply wp_NewSlice.
+  iIntros (ret) "Hret".
+  wp_loadField.
+  iDestruct (own_slice_small_read with "Hsl") as "(Hsl & Hsl_conv)".
+  iDestruct (own_slice_to_small with "Hret") as "Hret".
+
+  wp_apply (wp_SliceCopy_full_typed with "[$Hsl $Hret]").
+  {
+    iPureIntro.
+    rewrite replicate_length.
+    word.
+  }
+  iIntros "(Hsl & Hret)".
+  iDestruct ("Hsl_conv" with "Hsl") as "Hsl".
+
+  iDestruct (mono_list_auth_lb_valid with "[$] [$]") as %[_ Hpref].
+  iDestruct (mono_list_lb_own_get with "Hl_auth") as "#Hl_lb".
+  wp_loadField.
+  wp_apply (release_spec with "[-HΦ Hret $Hlk_inv $Hlocked]").
+  {
+    iExists _, _, _.
+    iFrame "#∗".
+  }
+
+  wp_pures.
+  iApply "HΦ".
+  by iFrame "#∗".
+Qed.
+
+End lib.
