src/program_proof/chat/full/proof.v
@@ -2,90 +2,11 @@ From Perennial.program_proof Require Import grove_prelude.
 From Goose.github_com.mit_pdos.secure_chat Require Import full.
 From iris.unstable.base_logic Require Import mono_list.
 From Perennial.algebra Require Import ghost_var.
-
-Context `{!heapGS Σ}.
-Context `{!ghost_varG Σ nat}.
-
-Module msgT.
-
-Record t :=
-  mk {
-    body: u64
-  }.
-
-Definition own (p : loc) (v : t) : iProp Σ :=
-  "Hbody" ∷ p ↦[msgT :: "body"] #v.(body).
-
-Global Instance IntoVal : IntoVal t.
-Proof.
-  refine {|
-    to_val := λ x, (#x.(body), #())%V;
-    from_val := λ x,
-      match x with
-      | (#(LitInt x'), #())%V => Some (mk x')
-      | _ => None
-      end;
-    IntoVal_def := mk 0;
-  |}.
-  intros []. auto.
-Defined.
-
-End msgT.
-
-Context `{!mono_listG msgT.t Σ}.
-
-Section chat_lib.
-
-Definition valid_chat (γ : gname) (P : list msgT.t → iProp Σ) : iProp Σ.
-Proof. Admitted.
-
-Global Instance valid_chat_persistent γ P : Persistent (valid_chat γ P).
-Proof. Admitted.
-
-Lemma wp_init (P : list msgT.t → iProp Σ) :
-  {{{ True }}}
-  Init #()
-  {{{
-    γ,
-    RET #();
-    mono_list_lb_own γ [] ∗
-    valid_chat γ P
-  }}}.
-Proof. Admitted.
-
-Lemma wp_put γ P p m l :
-  {{{
-    valid_chat γ P ∗
-    msgT.own p m ∗
-    mono_list_lb_own γ l ∗
-    (∀ l', ⌜l `prefix_of` l'⌝ -∗ □ P l' ={⊤}=∗ □ P (l' ++ [m]))
-  }}}
-  Put #p
-  {{{
-    RET #();
-    msgT.own p m
-  }}}.
-Proof. Admitted.
-
-Lemma wp_get γ P l :
-  {{{
-    valid_chat γ P ∗
-    mono_list_lb_own γ l
-  }}}
-  Get #()
-  {{{
-    (sl : Slice.t) (l' : list msgT.t),
-    RET (slice_val sl);
-    own_slice sl (structTy msgT) 1 l' ∗
-    mono_list_lb_own γ l' ∗
-    ⌜l `prefix_of` l'⌝ ∗
-    □ P l'
-  }}}.
-Proof. Admitted.
-
-End chat_lib.
+From Perennial.program_proof.chat.full Require Import lib.
 
 Section proof.
+
+Context `{!heapGS Σ, !ghost_varG Σ nat, !mono_listG msgT.t Σ}.
 
 Definition P γa γb (l : list msgT.t) : iProp Σ :=
   (⌜l = []⌝) ∨
@@ -93,195 +14,243 @@ Definition P γa γb (l : list msgT.t) : iProp Σ :=
   (⌜l = [msgT.mk 10; msgT.mk 11]⌝ ∗
     ghost_var γa DfracDiscarded 0 ∗ ghost_var γb DfracDiscarded 0).
 
-Lemma wp_alice (γa γb : gname) :
-  {{{ ghost_var γa (DfracOwn 1) 0 }}}
-  alice #()
+Ltac t_small :=
+  simpl in *;
+  word.
+
+Ltac t_shot :=
+  by iDestruct (ghost_var_valid_2 with "[$] [$]") as %[? _].
+
+Lemma wp_alice (γ γa γb : gname) cp l :
+  {{{
+    "#Hcli" ∷ is_ChatCli γ (P γa γb) cp ∗
+    "#Htriv_lb" ∷ mono_list_lb_own γ l ∗
+    "Hγ" ∷ ghost_var γa (DfracOwn 1) 0
+  }}}
+  alice #cp
   {{{ RET #(); True }}}.
 Proof.
   rewrite /alice.
-  iIntros (Φ) "Hγa HΦ".
-
-  wp_apply (wp_init (P γa γb)).
-  iIntros (γl) "[#Hl_lb #Hvalid]".
+  iIntros (Φ) "H HΦ".
+  iNamed "H".
 
   wp_apply wp_allocStruct; [val_ty|].
   iIntros (a) "Ha".
-  iDestruct (struct_fields_split with "Ha") as "HH".
-  iNamed "HH".
-  iRename "body" into "Ha".
+  iDestruct (struct_fields_split with "Ha") as "H".
+  iNamed "H".
+  iMod (readonly_alloc_1 with "body") as "#Ha".
 
   wp_apply wp_allocStruct; [val_ty|].
   iIntros (b) "Hb".
-  iDestruct (struct_fields_split with "Hb") as "HH".
-  iNamed "HH".
-  iRename "body" into "Hb".
+  iDestruct (struct_fields_split with "Hb") as "H".
+  iNamed "H".
+  iMod (readonly_alloc_1 with "body") as "#Hb".
 
-  wp_apply (wp_put with "[$Hvalid Ha $Hl_lb Hγa]").
+  wp_apply (wp_put with "[$Hcli $Htriv_lb Ha Hγ]").
   {
     instantiate (1:=msgT.mk _).
-    rewrite /msgT.own /P /=.
-    iFrame.
-    iIntros (?) "%Hpref #HP".
-    iDestruct "HP" as "[->|[[-> #Hro]|[-> [#Hro _]]]]".
+    iFrame "#".
+    iIntros (?) "% #HP".
+    iEval (rewrite /P) in "HP".
+    iDestruct "HP" as "[->|[[-> #Hro]|[-> [#Hro _]]]]"; [|t_shot|t_shot].
     {
-      iMod (ghost_var_persist with "Hγa") as "#Hγa".
-      iIntros "!>!>".
+      iMod (ghost_var_persist with "[$]") as "#Hγ".
       iRight.
       iLeft.
-      iSplit; [done|].
-      iAssumption.
+      by iFrame "#".
     }
-    (* TODO: `all:` or `1-2:` not working here for some reason. *)
-    1: by iDestruct (ghost_var_valid_2 with "Hγa Hro") as %[? _].
-    1: by iDestruct (ghost_var_valid_2 with "Hγa Hro") as %[? _].
   }
-  iIntros "Ha".
 
-  wp_apply (wp_get with "[$Hvalid $Hl_lb]").
-  iIntros (??) "(Hsl_own & #Hl_lb' & %Hpref & #HP)".
+  wp_apply (wp_get with "[$]").
+  iIntros (???) "{Htriv_lb} H".
+  iNamed "H".
+  clear Hpref.
   wp_apply wp_slice_len.
 
   wp_if_destruct.
   2: by iApply "HΦ".
 
-  iDestruct (own_slice_sz with "Hsl_own") as "%Hsz".
-  iDestruct (own_slice_to_small with "Hsl_own") as "Hsl_own".
+  iDestruct (own_slice_small_sz with "[$]") as %Hlen.
+  iDestruct (big_sepL2_length with "Hsep") as %Hlen'.
   rewrite /P.
-  iDestruct "HP" as "[->|[[-> _]|[-> _]]]".
-  1: replace (length _) with (0) in Hsz; [word|auto].
-  1: replace (length _) with (1) in Hsz; [word|auto].
-  replace (length _) with (2) in Hsz; [|auto].
+  iDestruct "HP" as "[->|[[-> _]|[-> _]]]"; [t_small|t_small|].
+  clear Hlen' Heqb0.
 
-  wp_apply (wp_SliceGet with "[$Hsl_own]"); [done|].
-  iIntros "Hsl_own".
-  rewrite /to_val.
-  rewrite /msgT.IntoVal.
-  wp_loadField.
+  iDestruct (big_sepL2_cons_inv_r with "Hsep") as (??) "{Hsep} [-> (Hsep0 & Hsep)]".
+  iDestruct (big_sepL2_cons_inv_r with "Hsep") as (? lnil) "{Hsep} [-> (Hsep1 & Hsep)]".
+  destruct lnil; [|done].
+  iClear "Hsep".
+
+  wp_apply (wp_SliceGet with "[$Hsl]"); [done|].
+  iIntros "Hsl".
+  wp_apply (wp_loadField_ro with "[$Hsep0]").
+  iClear "Hsep0".
+  wp_apply (wp_loadField_ro with "[$Ha]").
   wp_apply wp_Assert; [done|].
 
-  wp_apply (wp_SliceGet with "[$Hsl_own]"); [done|].
-  iIntros "Hsl_own".
-  wp_loadField.
+  wp_apply (wp_SliceGet with "[$Hsl]"); [done|].
+  iIntros "Hsl".
+  wp_apply (wp_loadField_ro with "[$Hsep1]").
+  iClear "Hsep1".
+  wp_apply (wp_loadField_ro with "[$Hb]").
   wp_apply wp_Assert; [done|].
 
   wp_apply wp_slice_len.
   wp_apply wp_Assert.
   {
-    (* TODO: should be simpler proof. *)
-    assert (U64 2 = sl.(Slice.sz)) by word.
-    rewrite <-H.
-    done.
+    simpl in *.
+    rewrite bool_decide_eq_true.
+    repeat f_equal.
+    word.
   }
+  iClear (Hlen) "Hsl".
 
-  wp_apply (wp_get with "[$Hvalid $Hl_lb']").
-  iIntros (??) "(Hsl_own' & _ & %Hpref' & #HP)".
-  rewrite /P.
-  iDestruct "HP" as "[->|[[-> _]|[-> _]]]".
-  {
-    (* TODO: should be simpler proof. *)
-    exfalso.
-    apply prefix_nil_inv in Hpref'.
-    discriminate Hpref'.
-  }
-  {
-    exfalso.
-    apply prefix_cons_inv_2 in Hpref'.
-    apply prefix_nil_inv in Hpref'.
-    discriminate Hpref'.
-  }
+  wp_apply (wp_get with "[$]").
+  iIntros (???) "{Hl_lb} H".
+  iNamed "H".
+  apply prefix_length in Hpref.
+  iDestruct "HP" as "[->|[[-> _]|[-> _]]]"; [t_small|t_small|].
+  iClear (Hpref) "Hl_lb".
 
-  iDestruct (own_slice_sz with "Hsl_own'") as "%Hsz'".
-  replace (length _) with (2) in Hsz'; [|auto].
-  iDestruct (own_slice_to_small with "Hsl_own'") as "Hsl_own'".
-  wp_apply (wp_SliceGet with "[$Hsl_own']"); [done|].
-  iIntros "Hsl_own'".
-  wp_loadField.
+  iDestruct (big_sepL2_cons_inv_r with "Hsep") as (??) "{Hsep} [-> (Hsep0 & Hsep)]".
+  iDestruct (big_sepL2_cons_inv_r with "Hsep") as (? lnil) "{Hsep} [-> (Hsep1 & Hsep)]".
+  destruct lnil; [|done].
+  iClear "Hsep".
+
+  wp_apply (wp_SliceGet with "[$Hsl]"); [done|].
+  iIntros "Hsl".
+  wp_apply (wp_loadField_ro with "[$Hsep0]").
+  iClear "Hsep0".
+  wp_apply (wp_loadField_ro with "[$Ha]").
   wp_apply wp_Assert; [done|].
 
-  wp_apply (wp_SliceGet with "[$Hsl_own']"); [done|].
-  iIntros "Hsl_own'".
-  wp_loadField.
+  wp_apply (wp_SliceGet with "[$Hsl]"); [done|].
+  iIntros "Hsl".
+  wp_apply (wp_loadField_ro with "[$Hsep1]").
+  iClear "Hsep1".
+  wp_apply (wp_loadField_ro with "[$Hb]").
+  wp_apply wp_Assert; [done|].
+
+  iDestruct (own_slice_small_sz with "[$]") as %Hlen.
+  wp_apply wp_slice_len.
+  wp_apply wp_Assert.
+  {
+    simpl in *.
+    rewrite bool_decide_eq_true.
+    repeat f_equal.
+    word.
+  }
+  iClear (Hlen) "Hsl".
+
+  wp_pures.
+  by iApply "HΦ".
+Qed.
+
+Lemma wp_bob (γ γa γb : gname) cp l :
+  {{{
+    "#Hcli" ∷ is_ChatCli γ (P γa γb) cp ∗
+    "#Htriv_lb" ∷ mono_list_lb_own γ l ∗
+    "Hγ" ∷ ghost_var γb (DfracOwn 1) 0
+  }}}
+  bob #cp
+  {{{ RET #(); True }}}.
+Proof.
+  rewrite /bob.
+  iIntros (Φ) "H HΦ".
+  iNamed "H".
+
+  wp_apply wp_allocStruct; [val_ty|].
+  iIntros (a) "Ha".
+  iDestruct (struct_fields_split with "Ha") as "H".
+  iNamed "H".
+  iMod (readonly_alloc_1 with "body") as "#Ha".
+
+  wp_apply wp_allocStruct; [val_ty|].
+  iIntros (b) "Hb".
+  iDestruct (struct_fields_split with "Hb") as "H".
+  iNamed "H".
+  iMod (readonly_alloc_1 with "body") as "#Hb".
+
+  wp_apply (wp_get with "[$]").
+  iIntros (???) "{Htriv_lb} H".
+  iNamed "H".
+  clear Hpref.
+  wp_apply wp_slice_len.
+
+  wp_if_destruct.
+  2: by iApply "HΦ".
+
+  iDestruct (own_slice_small_sz with "[$]") as %Hlen.
+  iDestruct (big_sepL2_length with "Hsep") as %Hlen'.
+  rewrite /P.
+  iDestruct "HP" as "[->|[[-> _]|[-> [_ #Hro]]]]"; [t_small|..|t_shot].
+  clear Hlen' Heqb0.
+
+  iDestruct (big_sepL2_cons_inv_r with "Hsep") as (? lnil) "{Hsep} [-> (Hsep0 & Hsep)]".
+  destruct lnil; [|done].
+  iClear "Hsep".
+
+  wp_apply (wp_SliceGet with "[$Hsl]"); [done|].
+  iIntros "Hsl".
+  wp_apply (wp_loadField_ro with "[$Hsep0]").
+  iClear "Hsep0".
+  wp_apply (wp_loadField_ro with "[$Ha]").
   wp_apply wp_Assert; [done|].
 
   wp_apply wp_slice_len.
   wp_apply wp_Assert.
   {
-    assert (U64 2 = sl0.(Slice.sz)) by word.
-    rewrite <-H.
-    done.
+    simpl in *.
+    rewrite bool_decide_eq_true.
+    repeat f_equal.
+    word.
+  }
+  iClear (Hlen) "Hsl".
+
+  wp_apply (wp_put with "[$Hcli $Hl_lb Hb Hγ]").
+  {
+    instantiate (1:=msgT.mk _).
+    iFrame "#".
+    iIntros (?) "%Hpref #HP".
+    apply prefix_length in Hpref.
+    iDestruct "HP" as "[->|[[-> #Hro]|[-> [_ #Hro]]]]"; [t_small|..|t_shot].
+    {
+      iMod (ghost_var_persist with "[$]") as "#Hγ".
+      iRight.
+      iRight.
+      by iFrame "#".
+    }
   }
 
   wp_pures.
   by iApply "HΦ".
 Qed.
 
-Lemma wp_bob (γa γb : gname) :
-  {{{ ghost_var γb (DfracOwn 1) 0 }}}
-  bob #()
+Lemma wp_main :
+  {{{ True }}}
+  main #()
   {{{ RET #(); True }}}.
-Proof.
-  rewrite /bob.
-  iIntros (Φ) "Hγb HΦ".
+Proof using ghost_varG0 heapGS0 mono_listG0 Σ.
+  rewrite /main.
+  iIntros (Φ) "_ HΦ".
+
+  iMod (ghost_var_alloc 0) as (γa) "Hγa".
+  iMod (ghost_var_alloc 0) as (γb) "Hγb".
 
   wp_apply (wp_init (P γa γb)).
-  iIntros (γl) "[#Hl_lb #Hvalid]".
-
-  wp_apply wp_allocStruct; [val_ty|].
-  iIntros (a) "Ha".
-  iDestruct (struct_fields_split with "Ha") as "HH".
-  iNamed "HH".
-  iRename "body" into "Ha".
-
-  wp_apply wp_allocStruct; [val_ty|].
-  iIntros (b) "Hb".
-  iDestruct (struct_fields_split with "Hb") as "HH".
-  iNamed "HH".
-  iRename "body" into "Hb".
-
-  wp_apply (wp_get with "[$Hvalid $Hl_lb]").
-  iIntros (??) "(Hsl_own & #Hl_lb' & %Hpref & #HP)".
-  wp_apply wp_slice_len.
-
-  wp_if_destruct.
-  2: by iApply "HΦ".
-
-  iDestruct (own_slice_sz with "Hsl_own") as "%Hsz".
-  iDestruct (own_slice_to_small with "Hsl_own") as "Hsl_own".
-  rewrite /P.
-  iDestruct "HP" as "[->|[[-> _]|[-> [_ #Hro]]]]".
-  1: replace (length _) with (0) in Hsz; [word|auto].
-  2: by iDestruct (ghost_var_valid_2 with "Hγb Hro") as %[? _].
-
-  wp_apply (wp_SliceGet with "[$Hsl_own]"); [done|].
-  iIntros "Hsl_own".
-  rewrite /to_val.
-  rewrite /msgT.IntoVal.
-  wp_loadField.
-  wp_apply wp_Assert; [done|].
-
-  wp_apply (wp_put with "[$Hvalid Hb $Hl_lb' Hγb]").
   {
-    instantiate (1:=msgT.mk _).
-    rewrite /msgT.own /P /=.
-    iFrame.
-    iIntros (?) "%Hpref' #HP".
-    iDestruct "HP" as "[->|[[-> #Hro]|[-> [_ #Hro]]]]".
-    {
-      exfalso.
-      apply prefix_nil_inv in Hpref'.
-      discriminate Hpref'.
-    }
-    2: by iDestruct (ghost_var_valid_2 with "Hγb Hro") as %[? _].
-    {
-      iMod (ghost_var_persist with "Hγb") as "#Hγb".
-      iIntros "!>!>".
-      iRight.
-      iRight.
-      iSplit; [done|].
-      iSplit; iAssumption.
-    }
+    rewrite /P.
+    naive_solver.
   }
-  iIntros "_".
+  iIntros (??) "H".
+  iNamed "H".
+
+  wp_apply (wp_fork with "[Hγa]").
+  {
+    iModIntro.
+    by wp_apply (wp_alice with "[$]").
+  }
+  wp_apply (wp_bob with "[$]").
 
   wp_pures.
   by iApply "HΦ".
